\documentclass{jlreq}
\usepackage{luatexja-fontspec}
\setmainfont{STIX Two Text}
\setsansfont{DejaVu Sans}
\setmonofont{0xProto}
\setmainjfont{YuKyo_Yoko-Medium}[BoldFont=YuKyo_Yoko-Bold]
\setsansjfont{YuGo-Medium}[BoldFont=YuGo-Bold]
\usepackage{mathtools}
\usepackage[warnings-off={mathtools-colon,mathtools-overbracket}]{unicode-math}
\unimathsetup{math-style=ISO,bold-style=ISO}
\setmathfont{STIX Two Math}
\mathtoolsset{showonlyrefs=true}
\usepackage[active,tightpage]{preview}
\newcommand{\ii}{\mathtt{i}}
\newcommand{\jj}{\mathtt{j}}
\newcommand{\kk}{\mathtt{k}}

\begin{document}

% 01
\begin{preview}
    \begin{equation}
        w + x \ii + y \jj + z \kk
    \end{equation}
\end{preview}

% 02
\begin{preview}
    \begin{gather}
        \ii^2 = -1 \quad / \quad \jj^2 = -1 \quad / \quad \kk^2 = -1 \\
        \ii \jj = \kk \quad / \quad \jj \kk = \ii \quad / \quad \kk \ii = \jj \quad / \quad \jj \ii = -\kk \quad / \quad \kk \jj = -\ii \quad / \quad \ii \kk = -\jj
    \end{gather}
\end{preview}

% 03
\begin{preview}
    \begin{align}
        (1 + 2 \ii + \jj + 4 \kk) + (5 + 3 \ii + 4 \jj - 2 \kk) & = 6 + 5 \ii + 5 \jj + 2 \kk \\
        (5 + 6 \ii + 2 \jj - 3 \kk) - (3 + 2 \ii + 3 \jj + \kk) & = 2 + 4 \ii - \jj - 4 \kk
    \end{align}
\end{preview}

% 04
\begin{preview}
    \begin{align}
        (1 + 2 \ii)(3 \jj + 4 \kk) & = 1 (3 \jj + 4 \kk) + 2 \ii (3 \jj + 4 \kk) \\
                                   & = 3 \jj + 4 \kk + 6 \ii \jj + 8 \ii \kk     \\
                                   & = 3 \jj + 4 \kk + 6 \kk - 8 \jj             \\
                                   & = -5 \jj + 10 \kk                           \\
        (3 \jj + 4 \kk)(1 + 2 \ii) & = 3 \jj (1 + 2 \ii) + 4 \kk (1 + 2 \ii)     \\
                                   & = 3 \jj + 6 \jj \ii + 4 \kk + 8 \kk \ii     \\
                                   & = 3 \jj - 6 \kk + 4 \kk + 8 \jj             \\
                                   & = 11 \jj - 2 \kk
    \end{align}
\end{preview}

% 05
\begin{preview}
    \begin{equation}
        (xz + x + y + z) \div (z + 1) = ?
    \end{equation}
\end{preview}

% 06
\begin{preview}
    \begin{equation}
        xz + x + y + z = (x + 1)(z + 1) + (y - 1)
    \end{equation}
\end{preview}

% 07
\begin{preview}
    \begin{equation}
        \frac{xz + x + y + z}{z + 1} = x + 1 + \frac{y - 1}{z + 1}
    \end{equation}
\end{preview}

% 08
\begin{preview}
    \begin{equation}
        w + x \ii + y \jj + z \kk
    \end{equation}
\end{preview}

% 09
\begin{preview}
    \begin{align}
        \alpha   & := w + x \ii + y \jj + z \kk  \\
        \alpha^* & :=  w - x \ii - y \jj - z \kk
    \end{align}
\end{preview}

% 10
\begin{preview}
    \begin{align}
        \alpha \alpha^* & = (w + x \ii + y \jj + z \kk)(w - x \ii - y \jj - z \kk)  \\
                        & = ww - wx \ii - wy \jj - wz \kk                           \\
                        & \quad + x \ii w - x \ii x \ii - x \ii y \jj - x \ii z \kk \\
                        & \quad + y \jj w - y \jj x \ii - y \jj y \jj - y \jj z \kk \\
                        & \quad + z \kk w - z \kk x \ii - z \kk y \jj - z \kk z \kk \\
                        & = w^2 - wx \ii - wy \jj - wz \kk                          \\
                        & \quad + wx \ii + x^2 - xy \kk + xz \jj                    \\
                        & \quad + wy \jj + xy \kk + y^2 - yz \ii                    \\
                        & \quad + wz \kk - xz \jj + yz \ii + z^2                    \\
                        & = w^2 + x^2 + y^2 + z^2
    \end{align}
\end{preview}

% 11
\begin{preview}
    \begin{align}
        |\alpha|   & := \sqrt{w^2 + x^2 + y^2 + z^2} \\
        |\alpha|^2 & = w^2 + x^2 + y^2 + z^2
    \end{align}
\end{preview}

% 12
\begin{preview}
    \begin{equation}
        \alpha \left(\frac{1}{|\alpha|^2} \alpha^*\right) = 1
    \end{equation}
\end{preview}

% 13
\begin{preview}
    \begin{align}
        (1 + 2 \ii + 3 \jj + 4 \kk) \div (1 - \ii + \jj + \kk) & = (1 + 2 \ii + 3 \jj + 4 \kk) (1 - \ii + \jj + \kk)^{-1}        \\
                                                               & = \frac{1}{4} (1 + 2 \ii + 3 \jj + 4 \kk) (1 + \ii - \jj - \kk) \\
                                                               & = \frac{1}{4} (6 + 4 \ii + 8 \jj - 2 \kk)                       \\
                                                               & = \frac{3}{2} + \ii + 2 \jj - \frac{1}{2} \kk
    \end{align}
\end{preview}

% 14
\begin{preview}
    \begin{equation}
        \cos \frac{\theta}{2} + (x_l \ii + y_l \jj + z_l \kk) \sin \frac{\theta}{2}
    \end{equation}
\end{preview}

% 15
\begin{preview}
    \begin{equation}
        \cos \frac{\theta}{2} + \ii \sin \frac{\theta}{2}
    \end{equation}
\end{preview}

% 16
\begin{preview}
    \begin{equation}
        \left( \cos \frac{\theta}{2} + \ii \sin \frac{\theta}{2} \right) \jj \left( \cos \frac{\theta}{2} - \ii \sin \frac{\theta}{2} \right)
    \end{equation}
\end{preview}

% 17
\begin{preview}
    \begin{align}
         & \left( \cos \frac{\theta}{2} + \ii \sin \frac{\theta}{2} \right) \jj \left( \cos \frac{\theta}{2} - \ii \sin \frac{\theta}{2} \right)                                           \\
         & = \jj \cos^2 \frac{\theta}{2} - \jj \ii \cos \frac{\theta}{2} \sin \frac{\theta}{2} + \ii \jj \sin \frac{\theta}{2} \cos \frac{\theta}{2} - \ii \jj \ii \sin^2 \frac{\theta}{2} \\
         & = \jj \cos^2 \frac{\theta}{2} + \kk \cos \frac{\theta}{2} \sin \frac{\theta}{2} + \kk \cos \frac{\theta}{2} \sin \frac{\theta}{2} - \jj \sin^2 \frac{\theta}{2}                 \\
         & = \jj \left( \cos^2 \frac{\theta}{2} - \sin^2 \frac{\theta}{2} \right) + \kk \left( 2 \cos \frac{\theta}{2} \sin \frac{\theta}{2} \right)                                       \\
         & = \jj \cos \theta + \kk \sin \theta
    \end{align}
\end{preview}

% 18
\begin{preview}
    \begin{equation}
        \frac{1}{\sqrt{2}} \jj + \frac{1}{\sqrt{2}} \kk = (0.7071 \dots) \jj + (0.7071 \dots) \kk
    \end{equation}
\end{preview}

\end{document}
